Separated the flat memory accessors. Removed the MC proofs from the compiler temporarily

x86/FlatAsm.v
@@ -11,6 +11,7 @@ Require Import Locations Stacklayout Conventions EraseArgs.
 Require Import Segment FlatAsmGlobenv FlatAsmBuiltin FlatAsmProgram.
 Require Import Asm RawAsm.
 Require Import Num.
+Require Import FlatMemAccessors.
 Require Globalenvs.
 
 
@@ -32,55 +33,6 @@ Section WITHEXTERNALCALLS.
 Context `{external_calls_prf: ExternalCalls}.
 
 Section RELSEM.
-
-
-Section WITHGE.
-
-Context {F V I: Type}.
-Variable ge: Genv.t F V I.
-  
-(** Evaluating an addressing mode *)
-
-Definition eval_addrmode32 (a: addrmode) (rs: regset) : val :=
-  let '(Addrmode base ofs const) := a in
-  Val.add  (match base with
-             | None => Vint Int.zero
-             | Some r => rs r
-            end)
-  (Val.add (match ofs with
-             | None => Vint Int.zero
-             | Some(r, sc) =>
-                if zeq sc 1
-                then rs r
-                else Val.mul (rs r) (Vint (Int.repr sc))
-             end)
-           (match const with
-            | inl ofs => Vint (Int.repr ofs)
-            | inr(id, ofs) => Genv.symbol_address ge id ofs
-            end)).
-
-Definition eval_addrmode64 (a: addrmode) (rs: regset) : val :=
-  let '(Addrmode base ofs const) := a in
-  Val.addl (match base with
-             | None => Vlong Int64.zero
-             | Some r => rs r
-            end)
-  (Val.addl (match ofs with
-             | None => Vlong Int64.zero
-             | Some(r, sc) =>
-                if zeq sc 1
-                then rs r
-                else Val.mull (rs r) (Vlong (Int64.repr sc))
-             end)
-           (match const with
-            | inl ofs => Vlong (Int64.repr ofs)
-            | inr(id, ofs) => Genv.symbol_address ge id ofs
-            end)).
-
-Definition eval_addrmode (a: addrmode) (rs: regset) : val :=
-  if Archi.ptr64 then eval_addrmode64 a rs else eval_addrmode32 a rs.
-
-End WITHGE.
 
 
 (** The semantics is purely small-step and defined as a function
@@ -107,43 +59,6 @@ Definition goto_label {F V I} (ge: Genv.t F V I) (fid:ident) (lbl: label) (rs: r
 (*     end *)
 (*   end. *)
 
-
-(** [CompCertiKOS:test-compcert-param-mem-accessors] For CertiKOS, we
-need to parameterize over [exec_load] and [exec_store], which will be
-defined differently depending on whether we are in kernel or user
-mode. *)
-
-Class MemAccessors
-      `{!Mem.MemoryModelOps mem}
-      (exec_load: forall F V I: Type, Genv.t F V I -> memory_chunk -> mem -> addrmode -> regset -> preg -> ptrofs -> outcome)
-      (exec_store: forall F V I: Type, Genv.t F V I -> memory_chunk -> mem -> addrmode -> regset -> preg -> list preg -> ptrofs -> outcome)
-: Prop := {}.
-
-Section MEM_ACCESSORS_DEFAULT.
-
-(** [CompCertiKOS:test-compcert-param-mem-accessors] Compcert does not
-care about kernel vs. user mode, and uses its memory model to define
-its memory accessors. *)
-
-Definition exec_load {F V I} (ge: Genv.t F V I) (chunk: memory_chunk) (m: mem)
-                     (a: addrmode) (rs: regset) (rd: preg) (sz:ptrofs):=
-  match Mem.loadv chunk m (eval_addrmode ge a rs) with
-  | Some v => Next (nextinstr_nf (rs#rd <- v) sz) m
-  | None => Stuck
-  end.
-
-Definition exec_store {F V I} (ge: Genv.t F V I) (chunk: memory_chunk) (m: mem)
-                      (a: addrmode) (rs: regset) (r1: preg)
-                      (destroyed: list preg) (sz:ptrofs) :=
-  match Mem.storev chunk m (eval_addrmode ge a rs) (rs r1) with
-  | Some m' =>
-    Next (nextinstr_nf (undef_regs destroyed rs) sz) m'
-  | None => Stuck
-  end.
-
-Local Instance mem_accessors_default: MemAccessors (@exec_load) (@exec_store).
-
-End MEM_ACCESSORS_DEFAULT.
 
 
 (** Execution of a single instruction [i] in initial state
